test/general/reverse_test.c
@@ -8,13 +8,17 @@ REQUIRES(pure (length arr == SizeT.v len))
 ENSURES(exists* s.arr |-> s)
 void reverse(ISARRAY(len) uint32_t *arr, size_t len) {
   size_t i = 0;
+  LEMMA(with varr. assert arr |-> varr);
+  LEMMA(with vlen. assert len |-> vlen);
   while (i < len / 2)
-    INVARIANTS( invariant c. ,
-                exists* vi. (i |->vi) ** (exists* s.arr |->s) ** pure (c == (vi `SizeT.lt` SizeT.div len 2sz)) 
-              ) 
+    INVARIANTS( invariant c.
+                (arr |-> varr) **
+                (len |-> vlen) ** (
+                exists* vi. (i |->vi) ** (exists* s. varr |->s) ** pure (c == (vi `SizeT.lt` SizeT.div vlen 2sz)) 
+              ) )
         {
                 size_t j = len - 1 - i;  
-                LEMMA(pts_to_len arr);
+                LEMMA(pts_to_len varr);
                 uint32_t tmp = arr[i];
                 arr[i] = arr[j];
                 arr[j] = tmp;
