test/issue-related/issue30_test.c
@@ -11,22 +11,90 @@ RETURNS(n : int32)
 ENSURES(x |->Frac px vx)
 ENSURES(y |->Frac py vy)
 ENSURES(pure(as_int n == max_spec(as_int vx)(as_int vy)))
-
+EXPECT_FAILURE() // see comments below
 int max_alt(int *x, int *y) {
+  LEMMA(let orig_x = x); // doesn't help, x is the local shadowed version
+  int result = 0;
+  int xx = *x;
+  int yy = *y;
+  LEMMA(with vx. assert x |-> vx);
+  LEMMA(with vy. assert y |-> vy);
+  LEMMA(with vxx. assert xx |-> vxx);
+  LEMMA(with vyy. assert yy |-> vyy);
+  if (xx > yy)
+    // Note: if does not frame anything, so the ensures must mention the full
+    // postcondition. But we need to mention the **original** x and y, not the
+    // locally shadowed versions, so we're out of luck here.
+    ENSURES(exists* r. (x |-> Frac px vx) ** (y |-> Frac py vy) ** (xx |-> vxx) ** 
+                       (yy |-> vyy) **
+                       (result |-> r) **
+                       pure (as_int r == max_spec (as_int vxx) (as_int vyy))
+           ) 
+    {
+      result = xx;
+    }
+    else {
+        result = yy;
+    }
+  return result;
+}
+
+// However, this now works without an ENSURES clause
+ERASED_ARG(#vx #vy : _)
+ERASED_ARG(#px #py : _)
+REQUIRES(x |->Frac px vx)
+REQUIRES(y |->Frac py vy)
+RETURNS(n : int32)
+ENSURES(x |->Frac px vx)
+ENSURES(y |->Frac py vy)
+ENSURES(pure(as_int n == max_spec(as_int vx)(as_int vy)))
+int max_alt2(int *x, int *y) {
   int result = 0;
   int vx = *x;
   int vy = *y;
   if (vx > vy)
-    ENSURES(exists* r. (x |->Frac px vx) ** 
-                       (y |->Frac py vy) **
-                       (result |->r) **
-                       pure (as_int r == max_spec (as_int vx) (as_int vy))
-           ) 
     {
       result = vx;
     }
     else {
         result = vy;
-    };
+    }
   return result;
+}
+
+// Or more naturally:
+ERASED_ARG(#vx #vy : _)
+ERASED_ARG(#px #py : _)
+REQUIRES(x |->Frac px vx)
+REQUIRES(y |->Frac py vy)
+RETURNS(n : int32)
+ENSURES(x |->Frac px vx)
+ENSURES(y |->Frac py vy)
+ENSURES(pure(as_int n == max_spec(as_int vx)(as_int vy)))
+int max_alt3(int *x, int *y) {
+  int result = 0;
+  if (*x > *y)
+    {
+      result = *x;
+    }
+    else {
+        result = *y;
+    }
+  return result;
+}
+
+// Or more naturally:
+ERASED_ARG(#vx #vy : _)
+ERASED_ARG(#px #py : _)
+REQUIRES(x |->Frac px vx)
+REQUIRES(y |->Frac py vy)
+RETURNS(n : int32)
+ENSURES(x |->Frac px vx)
+ENSURES(y |->Frac py vy)
+ENSURES(pure(as_int n == max_spec(as_int vx)(as_int vy)))
+int max_alt4(int *x, int *y) {
+  if (*x > *y)
+    return *x;
+  else
+    return *y;
 }
