test/issue-related/issue9_test.c
@@ -2,7 +2,8 @@
 #include "../include/PulseMacros.h"
 
 RETURNS(s:ref Pulse.Lib.C.Int32.int32)
-ENSURES(pure Pulse.Lib.C.Int32.(as_int s == 0))
+// ENSURES(pure Pulse.Lib.C.Int32.(as_int s == 0))
+// Now works but returns a dead ref
 int* refs_are_scoped()
 {
     int s = 0;
