test/snapshots/Issue30_test.fst
@@ -8,6 +8,7 @@ open Pulse.Lib.C
 
 
 let max_spec x y = if x < y then y else x
+[@@expect_failure]
 fn max_alt
 (x : ref Int32.t)
 (y : ref Int32.t)
@@ -20,17 +21,102 @@ ensures x |->Frac px vx
 ensures y |->Frac py vy
 ensures pure(as_int n == max_spec(as_int vx)(as_int vy))
 {
+let mut x : (ref Int32.t) = x;
+let mut y : (ref Int32.t) = y;
+let orig_x = x;
 let mut result : Int32.t = 0l;
-let vx : Int32.t = (! x);
-let vy : Int32.t = (! y);
-if((int32_to_bool (bool_to_int32 (Int32.gt vx vy))))
-ensures exists* r. (x |->Frac px vx) ** (y |->Frac py vy) ** (result |->r) ** pure (as_int r == max_spec (as_int vx) (as_int vy))
+let mut xx : Int32.t = (! (! x));
+let mut yy : Int32.t = (! (! y));
+with vx. assert x |-> vx;
+with vy. assert y |-> vy;
+with vxx. assert xx |-> vxx;
+with vyy. assert yy |-> vyy;
+if((int32_to_bool (bool_to_int32 (Int32.gt (! xx) (! yy)))))
+ensures exists* r. (x |-> Frac px vx) ** (y |-> Frac py vy) ** (xx |-> vxx) ** (yy |-> vyy) ** (result |-> r) ** pure (as_int r == max_spec (as_int vxx) (as_int vyy))
 {
-result := vx;
+result := (! xx);
 }
 else
 {
-result := vy;
+result := (! yy);
 };
 (! result);
+}
+
+fn max_alt2
+(x : ref Int32.t)
+(y : ref Int32.t)
+(#vx #vy : _)
+(#px #py : _)
+requires x |->Frac px vx
+requires y |->Frac py vy
+returns n : int32
+ensures x |->Frac px vx
+ensures y |->Frac py vy
+ensures pure(as_int n == max_spec(as_int vx)(as_int vy))
+{
+let mut x : (ref Int32.t) = x;
+let mut y : (ref Int32.t) = y;
+let mut result : Int32.t = 0l;
+let mut vx : Int32.t = (! (! x));
+let mut vy : Int32.t = (! (! y));
+if((int32_to_bool (bool_to_int32 (Int32.gt (! vx) (! vy)))))
+{
+result := (! vx);
+}
+else
+{
+result := (! vy);
+};
+(! result);
+}
+
+fn max_alt3
+(x : ref Int32.t)
+(y : ref Int32.t)
+(#vx #vy : _)
+(#px #py : _)
+requires x |->Frac px vx
+requires y |->Frac py vy
+returns n : int32
+ensures x |->Frac px vx
+ensures y |->Frac py vy
+ensures pure(as_int n == max_spec(as_int vx)(as_int vy))
+{
+let mut x : (ref Int32.t) = x;
+let mut y : (ref Int32.t) = y;
+let mut result : Int32.t = 0l;
+if((int32_to_bool (bool_to_int32 (Int32.gt (! (! x)) (! (! y))))))
+{
+result := (! (! x));
+}
+else
+{
+result := (! (! y));
+};
+(! result);
+}
+
+fn max_alt4
+(x : ref Int32.t)
+(y : ref Int32.t)
+(#vx #vy : _)
+(#px #py : _)
+requires x |->Frac px vx
+requires y |->Frac py vy
+returns n : int32
+ensures x |->Frac px vx
+ensures y |->Frac py vy
+ensures pure(as_int n == max_spec(as_int vx)(as_int vy))
+{
+let mut x : (ref Int32.t) = x;
+let mut y : (ref Int32.t) = y;
+if((int32_to_bool (bool_to_int32 (Int32.gt (! (! x)) (! (! y))))))
+{
+(! (! x));
+}
+else
+{
+(! (! y));
+};
 }
