test/snapshots/Issue9_test.fst
@@ -8,9 +8,8 @@ open Pulse.Lib.C
 
 
 fn refs_are_scoped ()
-returns s:Pulse.Lib.C.Int32.int32
-ensures pure Pulse.Lib.C.Int32.(as_int s == 0)
+returns s:ref Pulse.Lib.C.Int32.int32
 {
 let mut s : Int32.t = 0l;
-((! s));
+(s);
 }
