test/snapshots/Pulse_tutorial_loops.fst
@@ -12,18 +12,20 @@ fn count_down
 requires exists* v. (x |-> v) ** pure (as_int v >= 0)
 ensures x |-> 0l
 {
+let mut x : (ref Int32.t) = x;
 let mut keep_going : Int32.t = 1l;
+with vx. assert (x |-> vx);
 while((int32_to_bool (bool_to_int32 (Int32.eq (! keep_going) 1l)));
 )
-invariant b. exists* k v. (keep_going |-> k) ** (x |-> v) ** pure (as_int v >= 0) ** pure (b==(k=1l)) ** pure (k<>1l ==> v==0l)
+invariant b. exists* k v. (keep_going |-> k) ** (x |-> vx) ** (* tedious *) (vx |-> v) ** pure (as_int v >= 0) ** pure (b==(k=1l)) ** pure (k<>1l ==> v==0l)
 {
-if((int32_to_bool (bool_to_int32 (Int32.eq (! x) 0l))))
+if((int32_to_bool (bool_to_int32 (Int32.eq (! (! x)) 0l))))
 {
 keep_going := 0l;
 }
 else
 {
-x := (Int32.sub (! x) 1l);
+(! x) := (Int32.sub (! (! x)) 1l);
 };
 };}
 
@@ -35,14 +37,17 @@ requires pure (as_int x >= 0)
 returns i:int32
 ensures pure (as_int i == as_int x * as_int y)
 {
+let mut x : Int32.t = x;
+let mut y : Int32.t = y;
 let mut ctr : Int32.t = 0l;
 let mut acc : Int32.t = 0l;
-while((int32_to_bool (bool_to_int32 (Int32.lt (! ctr) x)));
+with vx vy. assert (x |-> vx) ** (y |-> vy);
+while((int32_to_bool (bool_to_int32 (Int32.lt (! ctr) (! x))));
 )
-invariant b. exists* c a. (ctr |-> c) ** (acc |-> a) ** pure (as_int c <= as_int x) ** pure (as_int a == (as_int c * as_int y)) ** pure (b == (as_int c < as_int x))
+invariant b. exists* c a. (x |-> vx) ** (y |-> vy) ** (* tedious *) (ctr |-> c) ** (acc |-> a) ** pure (as_int c <= as_int vx) ** pure (as_int a == (as_int c * as_int vy)) ** pure (b == (as_int c < as_int vx))
 {
 ctr := (Int32.add (! ctr) 1l);
-acc := (Int32.add (! acc) y);
+acc := (Int32.add (! acc) (! y));
 };(! acc);
 }
 
@@ -55,12 +60,14 @@ requires pure (fits ( * ) (as_int n) (as_int n + 1))
 returns i:int32
 ensures pure (as_int i == (as_int n * (as_int n + 1)) / 2)
 {
+let mut n : Int32.t = n;
 let mut acc : Int32.t = 0l;
 let mut ctr : Int32.t = 0l;
-sum_lemma(as_int n);
-while((int32_to_bool (bool_to_int32 (Int32.lt (! ctr) n)));
+sum_lemma(as_int !n);
+with vn. assert (n |-> vn);
+while((int32_to_bool (bool_to_int32 (Int32.lt (! ctr) (! n))));
 )
-invariant b. exists* c a. (ctr |-> c) ** (acc |-> a) ** pure (as_int c <= as_int n) ** pure (as_int c >= 0) ** pure (as_int c >= 0 ==> as_int a == sum (as_int c)) ** pure (b == (as_int c < as_int n))
+invariant b. exists* c a. (n |-> vn) ** (* tedious *) (ctr |-> c) ** (acc |-> a) ** pure (as_int c <= as_int vn) ** pure (as_int c >= 0) ** pure (as_int c >= 0 ==> as_int a == sum (as_int c)) ** pure (b == (as_int c < as_int vn))
 {
 ctr := (Int32.add (! ctr) 1l);
 acc := (Int32.add (! acc) (! ctr));
@@ -77,18 +84,22 @@ requires pure (as_int n > 0 ==> fib (as_int n) <= max_int32)
 requires exists* v0 v1. (cur |-> v0) ** (prev |-> v1)
 ensures exists* v0 v1. (cur |-> v0) ** (prev |-> v1) ** pure (as_int n > 0 ==> as_int v0 == fib (as_int n)) ** pure (as_int n > 0 ==> as_int v1 == fib (as_int n - 1))
 {
-if((int32_to_bool (bool_to_int32 (Int32.eq n 1l))))
+let mut n : Int32.t = n;
+let mut cur : (ref Int32.t) = cur;
+let mut prev : (ref Int32.t) = prev;
+if((int32_to_bool (bool_to_int32 (Int32.eq (! n) 1l))))
 {
-cur := 1l;
-prev := 1l;
+(! cur) := 1l;
+(! prev) := 1l;
 }
 else
 {
-fib_mono(as_int n) (as_int n - 1);
-(fib_rec (Int32.sub n 1l) cur prev);
-let tmp : Int32.t = (! cur);
-cur := (Int32.add (! cur) (! prev));
-prev := tmp;
+with vn. assert n |-> vn;
+fib_mono(as_int vn) (as_int vn - 1);
+(fib_rec (Int32.sub (! n) 1l) (! cur) (! prev));
+let mut tmp : Int32.t = (! (! cur));
+(! cur) := (Int32.add (! (! cur)) (! (! prev)));
+(! prev) := (! tmp);
 };
 }
 
@@ -99,8 +110,9 @@ requires pure (as_int n > 0 ==> fib (as_int n) <= max_int32)
 returns i:int32
 ensures pure (as_int n > 0 ==> as_int i == fib (as_int n))
 {
+let mut n : Int32.t = n;
 let mut cur : Int32.t = 0l;
 let mut prev : Int32.t = 0l;
-(fib_rec n cur prev);
+(fib_rec (! n) (cur) (prev));
 (! cur);
 }
