test/snapshots/Reverse_test.fst
@@ -15,16 +15,19 @@ requires exists* s.arr |-> s
 requires pure (length arr == SizeT.v len)
 ensures exists* s.arr |-> s
 {
+let mut arr : (array UInt32.t) = arr;
+let mut len : SizeT.t = len;
 let mut i : SizeT.t = (int32_to_sizet 0l);
-while((int32_to_bool (bool_to_int32 (SizeT.lt (! i) (SizeT.div len (int32_to_sizet 2l)))));
+with varr. assert arr |-> varr;
+with vlen. assert len |-> vlen;
+while((int32_to_bool (bool_to_int32 (SizeT.lt (! i) (SizeT.div (! len) (int32_to_sizet 2l)))));
 )
-invariant c. 
- exists* vi. (i |->vi) ** (exists* s.arr |->s) ** pure (c == (vi `SizeT.lt` SizeT.div len 2sz))
+invariant c. (arr |-> varr) ** (len |-> vlen) ** ( exists* vi. (i |->vi) ** (exists* s. varr |->s) ** pure (c == (vi `SizeT.lt` SizeT.div vlen 2sz)) )
 {
-let j : SizeT.t = (SizeT.sub (SizeT.sub len (int32_to_sizet 1l)) (! i));
-pts_to_len arr;
-let tmp : UInt32.t = (op_Array_Access arr (! i));
-arr.((! i)) <- (op_Array_Access arr j);
-arr.(j) <- tmp;
+let mut j : SizeT.t = (SizeT.sub (SizeT.sub (! len) (int32_to_sizet 1l)) (! i));
+pts_to_len varr;
+let mut tmp : UInt32.t = (op_Array_Access (! arr) (! i));
+(! arr).((! i)) <- (op_Array_Access (! arr) (! j));
+(! arr).((! j)) <- (! tmp);
 i := (SizeT.add (! i) (int32_to_sizet 1l));
 };}
